Primitive_Matchers/IpAddresses.thy
@@ -167,6 +167,15 @@ subsection{*IPv4 Addresses in IPTables Notation (how we parse it)*}
   lemma ipt_ipv4range_compress: "(\<Union> ip \<in> set (ipt_ipv4range_compress l). ipv4s_to_set ip) =
       (\<Inter> ip \<in> set (getPos l). ipv4s_to_set ip) - (\<Union> ip \<in> set (getNeg l). ipv4s_to_set ip)"
     by (metis wi_2_cidr_ipt_ipv4range_list comp_apply ipt_ipv4range_compress_def ipt_ipv4range_negation_type_to_br_intersect)
-      
+  
+  lemma wi_2_cidr_ipt_ipv4range_list_normalized_Ip4AddrNetmask: 
+    "\<forall>a'\<in>set (wi_2_cidr_ipt_ipv4range_list as). case a' of Ip4AddrNetmask x xa \<Rightarrow> True | _ \<Rightarrow> False"
+    apply(clarify)
+    apply(simp add: wi_2_cidr_ipt_ipv4range_list_def)
+    by force
+
+  lemma ipt_ipv4range_compress_normalized_Ip4AddrNetmask:
+    "\<forall>a'\<in>set (ipt_ipv4range_compress as). case a' of Ip4AddrNetmask x xa \<Rightarrow> True | _ \<Rightarrow> False"
+    by(simp add: ipt_ipv4range_compress_def wi_2_cidr_ipt_ipv4range_list_normalized_Ip4AddrNetmask)
 
 end
